code/hash/Hacl.Hash.MD.fsti
@@ -6,7 +6,7 @@ open Spec.Hash.Definitions
 module U32 = FStar.UInt32
 
 noextract inline_for_extraction
-val len_add32 (a: hash_alg{is_md a})
+val len_add32 (a: hash_alg{not (is_sha3 a)})
   (prev_len: len_t a)
   (input_len: U32.t { (U32.v input_len + len_v a prev_len) `less_than_max_input_length` a }):
   x:len_t a { len_v a x = len_v a prev_len + U32.v input_len }
